sha/verif_sha_update2.v
@@ -1,0 +1,289 @@
+Require Import floyd.proofauto.
+Require Import sha.sha.
+Require Import sha.SHA256.
+Require Import sha.spec_sha.
+Require Import sha.sha_lemmas.
+Local Open Scope nat.
+Local Open Scope logic.
+
+
+Lemma cVint_force_int_ZnthV:
+ forall sh contents hi, 
+  (hi <= Zlength contents)%Z ->
+  array_at tuchar sh (cVint (force_int oo ZnthV tuchar (map Vint contents))) 0 hi = 
+  array_at tuchar sh (ZnthV tuchar (map Vint contents)) 0 hi.
+Proof.
+unfold ZnthV; simpl.
+intros.
+apply array_at_ext; intros.
+unfold cVint,Basics.compose.
+if_tac. omega.
+assert (Z.to_nat i < length contents).
+apply Nat2Z.inj_lt.
+rewrite <- Zlength_correct; rewrite Z2Nat.id by omega.
+omega.
+clear - H2; revert contents H2; induction (Z.to_nat i); intros; destruct contents; 
+simpl in *; try omega; auto.
+apply IHn. omega.
+Qed.
+
+Definition update_inner_if :=
+              (Sifthenelse (Ebinop Oge (Etempvar _len tuint)
+                             (Etempvar _fragment tuint) tint)
+                (Ssequence
+                  (Ssequence
+                    (Scall (Some _ignore')
+                      (Evar _memcpy (Tfunction
+                                      (Tcons (tptr tvoid)
+                                        (Tcons (tptr tvoid)
+                                          (Tcons tuint Tnil))) (tptr tvoid)))
+                      ((Ebinop Oadd (Etempvar _p (tptr tuchar))
+                         (Etempvar _n tuint) (tptr tuchar)) ::
+                       (Etempvar _data (tptr tuchar)) ::
+                       (Etempvar _fragment tuint) :: nil))
+                    (Sset _ignore (Etempvar _ignore' (tptr tvoid))))
+                  (Ssequence
+                    (Scall None
+                      (Evar _sha256_block_data_order (Tfunction
+                                                       (Tcons
+                                                         (tptr t_struct_SHA256state_st)
+                                                         (Tcons (tptr tvoid)
+                                                           Tnil)) tvoid))
+                      ((Etempvar _c (tptr t_struct_SHA256state_st)) ::
+                       (Etempvar _p (tptr tuchar)) :: nil))
+                    (Ssequence
+                      (Sset _data
+                        (Ebinop Oadd (Etempvar _data (tptr tuchar))
+                          (Etempvar _fragment tuint) (tptr tuchar)))
+                      (Ssequence
+                        (Sset _len
+                          (Ebinop Osub (Etempvar _len tuint)
+                            (Etempvar _fragment tuint) tuint))
+                        (Ssequence
+                          (Scall (Some _ignore'1)
+                            (Evar _memset (Tfunction
+                                            (Tcons (tptr tvoid)
+                                              (Tcons tint (Tcons tuint Tnil)))
+                                            (tptr tvoid)))
+                            ((Etempvar _p (tptr tuchar)) ::
+                             (Econst_int (Int.repr 0) tint) ::
+                             (Ebinop Omul (Econst_int (Int.repr 16) tint)
+                               (Econst_int (Int.repr 4) tint) tint) :: nil))
+                          (Sset _ignore (Etempvar _ignore'1 (tptr tvoid))))))))
+                (Ssequence
+                  (Ssequence
+                    (Scall (Some _ignore'2)
+                      (Evar _memcpy (Tfunction
+                                      (Tcons (tptr tvoid)
+                                        (Tcons (tptr tvoid)
+                                          (Tcons tuint Tnil))) (tptr tvoid)))
+                      ((Ebinop Oadd (Etempvar _p (tptr tuchar))
+                         (Etempvar _n tuint) (tptr tuchar)) ::
+                       (Etempvar _data (tptr tuchar)) ::
+                       (Etempvar _len tuint) :: nil))
+                    (Sset _ignore (Etempvar _ignore'2 (tptr tvoid))))
+                  (Ssequence
+                    (Sassign
+                      (Efield
+                        (Ederef (Etempvar _c (tptr t_struct_SHA256state_st))
+                          t_struct_SHA256state_st) _num tuint)
+                      (Ebinop Oadd (Etempvar _n tuint)
+                        (Ecast (Etempvar _len tuint) tuint) tuint))
+                    (Sreturn None)))).
+
+Definition inv_at_inner_if sh hashed len c d dd data hi lo:=
+ (PROP ()
+   (LOCAL 
+   (`(eq (Vint (Int.repr (64- Zlength dd)))) (eval_id _fragment);
+   `(eq  (offset_val (Int.repr 40) c)) (eval_id _p);
+   `(eq (Vint (Int.repr (Zlength dd)))) (eval_id _n);
+   `(eq c) (eval_id _c); `(eq d) (eval_id _data);
+   `(eq (Vint (Int.repr (Z.of_nat len)))) (eval_id _len))
+   SEP  (`(array_at tuint Tsh (tuints (process_msg init_registers hashed)) 0 8 c);
+    `(sha256_length (hilo hi lo + (Z.of_nat len)*8) c);
+   `(array_at tuchar Tsh (ZnthV tuchar (map Vint (map Int.repr dd))) 0 64 (offset_val (Int.repr 40) c));
+   `(field_at Tsh t_struct_SHA256state_st _num (Vint (Int.repr (Zlength dd))) c);
+   K_vector;
+   `(data_block sh data d)))).
+
+Definition sha_update_inv sh hashed len c d (frag: list Z) (data: list Z) r_Nh r_Nl (done: bool) :=
+   (EX blocks:list int,
+   PROP  (len >= length blocks*4 - length frag /\
+              NPeano.divide LBLOCK (length blocks) /\ 
+              intlist_to_Zlist blocks = frag ++ firstn (length blocks * 4 - length frag) data /\
+             if done then len-(length blocks*4 - length frag) < CBLOCK else True)
+   LOCAL  (`(eq (offset_val (Int.repr 40) c)) (eval_id _p);
+   `(eq c) (eval_id _c); `(eq (offset_val (Int.repr (Z.of_nat (length blocks*4-length frag))) d)) (eval_id _data);
+   `(eq (Vint (Int.repr (Z.of_nat (len- (length blocks*4 - length frag)))))) (eval_id _len))
+   SEP  (K_vector;
+    `(array_at tuint Tsh (tuints (process_msg init_registers (hashed ++ blocks))) 0 8 c);
+    `(sha256_length (hilo r_Nh r_Nl + (Z.of_nat len)*8) c);
+   `(array_at_ tuchar Tsh 0 64 (offset_val (Int.repr 40) c));
+   `(field_at_ Tsh t_struct_SHA256state_st _num c);
+   `(data_block sh data d))).
+
+Lemma update_inner_if_proof:
+ forall (Espec: OracleKind) (hashed: list int) (dd data: list Z)
+            (c d: val) (sh: share) (len: nat) (hi lo: int)
+ (H: len <= length data)
+ (H7 : ((Zlength hashed * 4 + Zlength dd) * 8)%Z = hilo hi lo)
+ (H3 : length dd < CBLOCK)
+ (H3' : Forall isbyteZ dd)
+ (H4 : NPeano.divide LBLOCK (length hashed))
+ (Hlen : (Z.of_nat len <= Int.max_unsigned)%Z),
+semax
+  (initialized _fragment  (initialized _p
+     (initialized _n
+        (initialized _data (func_tycontext f_SHA256_Update Vprog Gtot)))))
+  (inv_at_inner_if sh hashed len c d dd data hi lo)
+  update_inner_if
+  (overridePost (sha_update_inv sh hashed len c d dd data hi lo false)
+     (function_body_ret_assert tvoid
+        (EX  a' : s256abs,
+         PROP  (update_abs (firstn len data) (S256abs hashed dd) a')
+         LOCAL ()
+         SEP  (K_vector; `(sha256state_ a' c); `(data_block sh data d))))).
+Proof.
+intros.
+name c' _c.
+name data_ _data_.
+name len' _len.
+name data' _data.
+name p _p.
+name n _n.
+name fragment_ _fragment.
+simplify_Delta.
+unfold sha_update_inv, inv_at_inner_if, update_inner_if.
+abbreviate_semax.
+rewrite semax_seq_skip.
+ set (j := (40 + Zlength dd)%Z).
+ set (k := (64-Zlength dd)%Z).
+assert (0 < k <= 64)%Z
+ by (unfold k; clear - H3;
+     apply Nat2Z.inj_lt in H3; rewrite Zlength_correct;
+    change (Z.of_nat CBLOCK) with 64%Z in *;
+    omega).
+ assert (64 < Int.max_unsigned)%Z
+  by (compute; reflexivity).
+apply Nat2Z.inj_le in H; rewrite <- Zlength_correct in H.
+unfold data_block; simpl. normalize.
+rename H2 into DBYTES.
+forward_if (sha_update_inv sh hashed len c d dd data hi lo false).
+ + entailer!.  (* cond-expression typechecks *)
+ + (* then clause: len >= fragment *)
+  simpl typeof.
+  unfold K_vector.
+  apply (remember_value (eval_id _fragment)); intro fragment.
+  forward. (* ignore = memcpy (p+n,data,fragment); *)
+  simpl split. simpl @snd.
+  instantiate (1:=((sh,Tsh), 
+                           offset_val (Int.repr (Zlength dd)) (offset_val (Int.repr 40) c),
+                           d, 
+                           Int.unsigned (force_int fragment),
+                           Basics.compose force_int (ZnthV tuchar (map Vint (map Int.repr data)))))
+        in (Value of witness).
+  unfold witness. 
+ normalize.
+ fold j; fold k.
+ entailer!.
+ rewrite H6; reflexivity.
+ clear POSTCONDITION MORE_COMMANDS.
+ unfold witness in *; clear witness. clear fragment H5.
+ rewrite negb_true_iff in H6. 
+ apply ltu_repr_false in H6; [ | repable_signed | omega].
+ clear TC TC1 TC0.
+ unfold j,k in *; clear j k.
+rewrite cVint_force_int_ZnthV
+ by (rewrite initial_world.Zlength_map; omega).
+ rewrite memory_block_array_tuchar by omega.
+ rewrite (split_array_at (Zlength dd) _ _ (ZnthV tuchar (map Vint (map Int.repr dd))))
+    by omega.
+ rewrite (split_array_at (64-Zlength dd) _ _ (tuchars (map Int.repr data)))
+    by omega.
+ replace (offset_val (Int.repr (40 + Zlength dd)) c)
+          with (offset_val (Int.repr (sizeof tuchar * Zlength dd)) (offset_val (Int.repr 40) c))
+  by (change (sizeof tuchar) with 1%Z; rewrite Z.mul_1_l; rewrite offset_offset_val, add_repr; auto).
+rewrite <- offset_val_array_at_.
+  rewrite Z.add_0_r.
+  replace (Zlength dd + (64-Zlength dd))%Z with 64%Z by omega.
+ cancel.
+ cbv beta iota.
+ autorewrite with norm subst.
+ forward. (* finish the call *)
+ admit.
+ + (* else clause: len < fragment *)
+   simpl typeof; unfold K_vector.
+   forward. (* ignore'2 := memcpy (p+n, data, len); *)
+  simpl split. simpl @snd.
+  instantiate (1:=((sh,Tsh), 
+                           offset_val (Int.repr (Zlength dd)) (offset_val (Int.repr 40) c),
+                           d, 
+                           Z.of_nat len,
+                           Basics.compose force_int (ZnthV tuchar (map Vint (map Int.repr data)))))
+        in (Value of witness).
+  unfold witness. 
+ normalize.
+ clear POSTCONDITION MORE_COMMANDS.
+ fold j; fold k.
+ entailer!.
+ rewrite H5; reflexivity.
+ rewrite cVint_force_int_ZnthV
+ by (rewrite initial_world.Zlength_map; omega).
+ rewrite negb_false_iff in H5.
+ apply ltu_repr in H5; [ | repable_signed | omega].
+ unfold j,k in *; clear j k.
+ replace (offset_val (Int.repr (40 + Zlength dd)) c)
+          with (offset_val (Int.repr (sizeof tuchar * Zlength dd)) (offset_val (Int.repr 40) c))
+  by (change (sizeof tuchar) with 1%Z; rewrite Z.mul_1_l; rewrite offset_offset_val, add_repr; auto).
+
+ rewrite memory_block_array_tuchar';  [ | destruct c; try contradiction Pc; apply I | omega].
+ rewrite <- offset_val_array_at_.
+  rewrite Z.add_0_r.
+ unfold tuchars.
+ rewrite (split_array_at (Zlength dd) _ _ (ZnthV tuchar (map Vint (map Int.repr dd))))
+    by omega.
+ rewrite (split_array_at (Zlength dd + Z.of_nat len) _ _ (ZnthV tuchar (map Vint (map Int.repr dd)))
+                              (Zlength dd))
+    by omega.
+ rewrite (split_array_at (Z.of_nat len) _ _ (tuchars (map Int.repr data)))
+    by omega.
+ unfold tuchars.
+ cancel.
+ cbv beta iota.
+ autorewrite with norm subst.
+ forward. (* finish the call *)
+ forward. (* c->num = n+(unsigned int)len; *)
+ fold j; fold k.
+ forward. (* return; *)
+ apply exp_right with (S256abs hashed (dd ++ firstn len data)).
+ unfold id.
+ unfold data_block.
+ unfold K_vector.
+ repeat rewrite TT_andp.
+ rewrite cVint_force_int_ZnthV
+ by (rewrite initial_world.Zlength_map; omega).
+rewrite array_at_tuchar_isbyteZ. 
+ rewrite (prop_true_andp (Forall _ data)) by auto.
+ rewrite negb_false_iff in H5.
+ apply ltu_repr in H5; [ | repable_signed | omega].
+ clear TC1 TC TC3 TC2 TC0.
+ unfold k in H0,H5.
+ rewrite (prop_true_andp (_ /\ _)).
+Focus 2. {
+ split; auto.
+ rewrite (app_nil_end hashed) at 2.
+ apply (Update_abs _ hashed nil dd (dd++firstn len data)); auto.
+ rewrite app_length. rewrite firstn_length. rewrite min_l.
+ apply Nat2Z.inj_lt. rewrite Nat2Z.inj_add.
+ rewrite <- Zlength_correct. change (Z.of_nat CBLOCK) with 64%Z.
+ omega.
+ apply Nat2Z.inj_le; rewrite <- Zlength_correct; assumption.
+ exists 0. reflexivity.
+} Unfocus.
+ unfold sha256state_.
+ normalize. clear H8.
+ admit. (* getting there *)
+ + forward. (* bogus skip *)
+    rewrite overridePost_normal'.
+    apply andp_left2; auto.
+Qed.
